Migrate NFA.Path to ValidPos

correctness/RegexCorrectness/NFA/Semantics/Path.lean
@@ -12,180 +12,109 @@ open String (ValidPos)
 
 namespace Regex.NFA
 
+@[grind]
 inductive Step {s : String} (nfa : NFA) (lb : Nat) : Nat → ValidPos s → Nat → ValidPos s → Option (Nat × ValidPos s) → Prop where
-  | epsilon {i j it} (ge : lb ≤ i) (lt : i < nfa.nodes.size) (eq : nfa[i] = .epsilon j) (v : it.Valid) :
-    Step nfa lb i it j it .none
-  | anchor {i j it a} (ge : lb ≤ i) (lt : i < nfa.nodes.size) (eq : nfa[i] = .anchor a j) (v : it.Valid) (h : a.test it) :
-    Step nfa lb i it j it .none
-  | splitLeft {i j₁ j₂ it} (ge : lb ≤ i) (lt : i < nfa.nodes.size) (eq : nfa[i] = .split j₁ j₂) (v : it.Valid) :
-    Step nfa lb i it j₁ it .none
-  | splitRight {i j₁ j₂ it} (ge : lb ≤ i) (lt : i < nfa.nodes.size) (eq : nfa[i] = .split j₁ j₂) (v : it.Valid) :
-    Step nfa lb i it j₂ it .none
-  | save {i j it offset} (ge : lb ≤ i) (lt : i < nfa.nodes.size) (eq : nfa[i] = .save offset j) (v : it.Valid) :
-    Step nfa lb i it j it (.some (offset, it.pos))
-  | char {i j it l c r} (ge : lb ≤ i) (lt : i < nfa.nodes.size) (eq : nfa[i] = .char c j) (vf : it.ValidFor l (c :: r)) :
-    Step nfa lb i it j it.next .none
-  | sparse {i j it l c r cs} (ge : lb ≤ i) (lt : i < nfa.nodes.size) (eq : nfa[i] = .sparse cs j) (vf : it.ValidFor l (c :: r)) (mem : c ∈ cs):
-    Step nfa lb i it j it.next .none
+  | epsilon {i j p} (ge : lb ≤ i) (lt : i < nfa.nodes.size) (eq : nfa[i] = .epsilon j) :
+    Step nfa lb i p j p .none
+  | anchor {i j p a} (ge : lb ≤ i) (lt : i < nfa.nodes.size) (eq : nfa[i] = .anchor a j) (h : a.test p) :
+    Step nfa lb i p j p .none
+  | splitLeft {i j₁ j₂ p} (ge : lb ≤ i) (lt : i < nfa.nodes.size) (eq : nfa[i] = .split j₁ j₂) :
+    Step nfa lb i p j₁ p .none
+  | splitRight {i j₁ j₂ p} (ge : lb ≤ i) (lt : i < nfa.nodes.size) (eq : nfa[i] = .split j₁ j₂) :
+    Step nfa lb i p j₂ p .none
+  | save {i j p offset} (ge : lb ≤ i) (lt : i < nfa.nodes.size) (eq : nfa[i] = .save offset j) :
+    Step nfa lb i p j p (.some (offset, p))
+  | char {i j p c} (ge : lb ≤ i) (lt : i < nfa.nodes.size) (eq : nfa[i] = .char c j) (ne : p ≠ s.endValidPos) (eq' : p.get ne = c) :
+    Step nfa lb i p j (p.next ne) .none
+  | sparse {i j p cs} (ge : lb ≤ i) (lt : i < nfa.nodes.size) (eq : nfa[i] = .sparse cs j) (ne : p ≠ s.endValidPos) (mem : p.get ne ∈ cs):
+    Step nfa lb i p j (p.next ne) .none
 
 namespace Step
 
-variable {nfa nfa' : NFA} {lb lb' i it j it' update}
+variable {s : String} {nfa nfa' : NFA} {lb lb'} {p p' : ValidPos s} {i j k update}
 
-theorem ge (step : nfa.Step lb i it j it' update) : lb ≤ i := by
+theorem ge (step : nfa.Step lb i p j p' update) : lb ≤ i := by
   cases step <;> assumption
 
-theorem lt (step : nfa.Step lb i it j it' update) : i < nfa.nodes.size := by
+theorem lt (step : nfa.Step lb i p j p' update) : i < nfa.nodes.size := by
   cases step <;> assumption
 
-theorem lt_right (wf : nfa.WellFormed) (step : nfa.Step lb i it j it' update) : j < nfa.nodes.size := by
+theorem lt_right (wf : nfa.WellFormed) (step : nfa.Step lb i p j p' update) : j < nfa.nodes.size := by
   have inBounds := wf.inBounds ⟨i, step.lt⟩
   cases step <;> simp_all [Node.inBounds]
 
-theorem it_eq_or_next (step : nfa.Step lb i it j it' update) : it' = it ∨ (it.hasNext ∧ it' = it.next) := by
-  cases step
-  case char _ _ _ vf _ => simp [vf.hasNext]
-  case sparse _ _ _ vf _ => simp [vf.hasNext]
-  all_goals simp
+theorem eq_or_next (step : nfa.Step lb i p j p' update) : p' = p ∨ ∃ ne : p ≠ s.endValidPos, p' = p.next ne := by
+  cases step <;> simp_all
 
-theorem le_pos (step : nfa.Step lb i it j it' update) : it.pos ≤ it'.pos := by
-  cases step.it_eq_or_next with
-  | inl eq => exact eq ▸ Nat.le_refl _
-  | inr eq =>
-    simp only [Iterator.pos, eq, Iterator.next, String.Pos.Raw.next]
-    exact Nat.le_add_right _ _
+theorem le (step : nfa.Step lb i p j p' update) : p ≤ p' := by
+  match step.eq_or_next with
+  | .inl eq => exact eq ▸ ValidPos.le_refl _
+  | .inr ⟨_, eq⟩ => exact ValidPos.le_of_lt (eq ▸ ValidPos.lt_next p)
 
-theorem validL (step : nfa.Step lb i it j it' update) : it.Valid := by
-  cases step
-  case char _ _ _ vf _ => exact vf.valid
-  case sparse _ _ _ vf _ => exact vf.valid
-  all_goals assumption
-
-theorem validR (step : nfa.Step lb i it j it' update) : it'.Valid := by
-  cases step
-  case char _ _ _ vf _ => exact vf.next.valid
-  case sparse _ _ _ vf _ => exact vf.next.valid
-  all_goals assumption
-
-theorem toString_eq (step : nfa.Step lb i it j it' update) :
-  it'.toString = it.toString := by
-  cases step.it_eq_or_next with
-  | inl eq => simp [eq]
-  | inr eq => simp [eq, String.Iterator.next, String.Pos.Raw.next]
-
-theorem le_endPos (step : nfa.Step lb i it j it' update) : it'.pos ≤ it.toString.endPos :=
-  step.toString_eq ▸ step.validR.le_endPos
-
-theorem cast (step : nfa.Step lb i it j it' update)
+theorem cast (step : nfa.Step lb i p j p' update)
   {lt : i < nfa'.nodes.size} (h : nfa[i]'step.lt = nfa'[i]) :
-  nfa'.Step lb i it j it' update := by
+  nfa'.Step lb i p j p' update := by
   cases step with
-  | epsilon ge _ eq v => exact .epsilon ge lt (h ▸ eq) v
-  | anchor ge _ eq v h' => exact .anchor ge lt (h ▸ eq) v h'
-  | splitLeft ge _ eq v => exact .splitLeft ge lt (h ▸ eq) v
-  | splitRight ge _ eq v => exact .splitRight ge lt (h ▸ eq) v
-  | save ge _ eq v => exact .save ge lt (h ▸ eq) v
-  | char ge _ eq v => exact .char ge lt (h ▸ eq) v
-  | sparse ge _ eq v mem => exact .sparse ge lt (h ▸ eq) v mem
+  | epsilon ge _ eq => exact .epsilon ge lt (h ▸ eq)
+  | anchor ge _ eq h' => exact .anchor ge lt (h ▸ eq) h'
+  | splitLeft ge _ eq => exact .splitLeft ge lt (h ▸ eq)
+  | splitRight ge _ eq => exact .splitRight ge lt (h ▸ eq)
+  | save ge _ eq => exact .save ge lt (h ▸ eq)
+  | char ge _ eq ne eq' => exact .char ge lt (h ▸ eq) ne eq'
+  | sparse ge _ eq ne mem => exact .sparse ge lt (h ▸ eq) ne mem
 
-theorem liftBound' (ge : lb' ≤ i) (step : nfa.Step lb i it j it' update) :
-  nfa.Step lb' i it j it' update := by
+theorem liftBound' (ge : lb' ≤ i) (step : nfa.Step lb i p j p' update) :
+  nfa.Step lb' i p j p' update := by
   cases step with
-  | epsilon _ lt eq v => exact .epsilon ge lt eq v
-  | anchor _ lt eq h v => exact .anchor ge lt eq h v
-  | splitLeft _ lt eq v => exact .splitLeft ge lt eq v
-  | splitRight _ lt eq v => exact .splitRight ge lt eq v
-  | save _ lt eq v => exact .save ge lt eq v
-  | char _ lt eq v => exact .char ge lt eq v
-  | sparse _ lt eq v mem => exact .sparse ge lt eq v mem
+  | epsilon _ lt eq => exact .epsilon ge lt eq
+  | anchor _ lt eq h => exact .anchor ge lt eq h
+  | splitLeft _ lt eq => exact .splitLeft ge lt eq
+  | splitRight _ lt eq => exact .splitRight ge lt eq
+  | save _ lt eq => exact .save ge lt eq
+  | char _ lt eq ne eq' => exact .char ge lt eq ne eq'
+  | sparse _ lt eq ne mem => exact .sparse ge lt eq ne mem
 
-theorem liftBound (le : lb' ≤ lb) (step : nfa.Step lb i it j it' update) :
-  nfa.Step lb' i it j it' update :=
+theorem liftBound (le : lb' ≤ lb) (step : nfa.Step lb i p j p' update) :
+  nfa.Step lb' i p j p' update :=
   step.liftBound' (Nat.le_trans le step.ge)
 
 theorem iff_done {lt : i < nfa.nodes.size} (eq : nfa[i] = .done) :
-  nfa.Step lb i it j it' update ↔ False := by
+  nfa.Step lb i p j p' update ↔ False := by
   apply Iff.intro
   . intro step
     cases step <;> simp_all
   . simp
 
 theorem iff_fail {lt : i < nfa.nodes.size} (eq : nfa[i] = .fail) :
-  nfa.Step lb i it j it' update ↔ False := by
-  apply Iff.intro
-  . intro step
-    cases step <;> simp_all
-  . simp
+  nfa.Step lb i p j p' update ↔ False := by
+  grind
 
 theorem iff_epsilon {next} {lt : i < nfa.nodes.size} (eq : nfa[i] = .epsilon next) :
-  nfa.Step lb i it j it' update ↔ lb ≤ i ∧ j = next ∧ it' = it ∧ update = .none ∧ it.Valid := by
-  apply Iff.intro
-  . intro step
-    cases step <;> simp_all
-  . intro ⟨ge, hj, hit, hupdate, v⟩
-    simp_all
-    exact .epsilon ge lt eq v
+  nfa.Step lb i p j p' update ↔ lb ≤ i ∧ j = next ∧ p' = p ∧ update = .none := by
+  grind
 
 theorem iff_anchor {anchor next} {lt : i < nfa.nodes.size} (eq : nfa[i] = .anchor anchor next) :
-  nfa.Step lb i it j it' update ↔ lb ≤ i ∧ j = next ∧ it' = it ∧ update = .none ∧ it.Valid ∧ anchor.test it := by
-  apply Iff.intro
-  . intro step
-    cases step <;> simp_all
-  . intro ⟨ge, hj, hit, hupdate, v, htest⟩
-    simp_all
-    exact .anchor ge lt eq v htest
+  nfa.Step lb i p j p' update ↔ lb ≤ i ∧ j = next ∧ p' = p ∧ update = .none ∧ anchor.test p := by
+  grind
 
 theorem iff_split {next₁ next₂} {lt : i < nfa.nodes.size} (eq : nfa[i] = .split next₁ next₂) :
-  nfa.Step lb i it j it' update ↔ lb ≤ i ∧ (j = next₁ ∨ j = next₂) ∧ it' = it ∧ update = .none ∧ it.Valid := by
-  apply Iff.intro
-  . intro step
-    cases step <;> simp_all
-  . intro ⟨ge, hj, hit, hupdate, v⟩
-    cases hj with
-    | inl hj =>
-      simp_all
-      exact .splitLeft ge lt eq v
-    | inr hj =>
-      simp_all
-      exact .splitRight ge lt eq v
+  nfa.Step lb i p j p' update ↔ lb ≤ i ∧ (j = next₁ ∨ j = next₂) ∧ p' = p ∧ update = .none := by
+  grind
 
 theorem iff_save {offset next} {lt : i < nfa.nodes.size} (eq : nfa[i] = .save offset next) :
-  nfa.Step lb i it j it' update ↔ lb ≤ i ∧ j = next ∧ it' = it ∧ update = .some (offset, it.pos) ∧ it.Valid := by
-  apply Iff.intro
-  . intro step
-    cases step <;> simp_all
-  . intro ⟨ge, hj, hit, hupdate, v⟩
-    simp_all
-    exact .save ge lt eq v
+  nfa.Step lb i p j p' update ↔ lb ≤ i ∧ j = next ∧ p' = p ∧ update = .some (offset, p) := by
+  grind
 
 theorem iff_char {c next} {lt : i < nfa.nodes.size} (eq : nfa[i] = .char c next) :
-  nfa.Step lb i it j it' update ↔ ∃ l r, lb ≤ i ∧ j = next ∧ it' = it.next ∧ update = .none ∧ it.ValidFor l (c :: r) := by
-  apply Iff.intro
-  . intro step
-    cases step
-    case char l c r ge lt vf v =>
-      simp_all
-      exact ⟨l, r, vf⟩
-    all_goals simp_all
-  . intro ⟨l, r, ge, hj, hit, hupdate, vf⟩
-    simp_all
-    exact .char ge lt eq vf
+  nfa.Step lb i p j p' update ↔ ∃ ne, lb ≤ i ∧ j = next ∧ p' = p.next ne ∧ update = .none ∧ p.get ne = c := by
+  grind
 
 theorem iff_sparse {cs next} {lt : i < nfa.nodes.size} (eq : nfa[i] = .sparse cs next) :
-  nfa.Step lb i it j it' update ↔ ∃ l c r, lb ≤ i ∧ j = next ∧ it' = it.next ∧ update = .none ∧ it.ValidFor l (c :: r) ∧ c ∈ cs := by
-  apply Iff.intro
-  . intro step
-    cases step
-    case sparse l c r cs ge lt mem vf hn =>
-      simp [eq] at hn
-      exact ⟨l, c, r, ge, by simp [hn.2], rfl, rfl, vf, hn.1 ▸ mem⟩
-    all_goals simp_all
-  . intro ⟨l, c, r, ge, hj, hit, hupdate, vf, mem⟩
-    simp_all
-    exact .sparse ge lt eq vf mem
+  nfa.Step lb i p j p' update ↔ ∃ ne, lb ≤ i ∧ j = next ∧ p' = p.next ne ∧ update = .none ∧ p.get ne ∈ cs := by
+  grind
 
-theorem compile_liftBound {e nfa} (eq : compile e = nfa) (step : nfa.Step 0 i it j it' update) :
-  nfa.Step 1 i it j it' update := by
+theorem compile_liftBound {e nfa} (eq : compile e = nfa) (step : nfa.Step 0 i p j p' update) :
+  nfa.Step 1 i p j p' update := by
   cases Nat.eq_zero_or_pos i with
   | inl eqi =>
     have lt : i < nfa.nodes.size := eqi ▸ lt_zero_size_compile eq
@@ -196,58 +125,44 @@ theorem compile_liftBound {e nfa} (eq : compile e = nfa) (step : nfa.Step 0 i it
 end Step
 
 /--
-A collection of steps in an NFA forms a path.
+A collection of steps in an NFA forms a path. The path must contain at least one step
+(which implies that the first state is greater than or equal to the lower bound).
 -/
-inductive Path (nfa : NFA) (lb : Nat) : Nat → Iterator → Nat → Iterator → List (Nat × String.Pos.Raw) → Prop where
-  | last {i it j it' update} (step : Step nfa lb i it j it' update) : Path nfa lb i it j it' (List.ofOption update)
-  | more {i it j it' k it'' update updates} (step : Step nfa lb i it j it' update) (rest : Path nfa lb j it' k it'' updates) :
-    Path nfa lb i it k it'' (update ::ₒ updates)
+inductive Path {s : String} (nfa : NFA) (lb : Nat) : Nat → ValidPos s → Nat → ValidPos s → List (Nat × ValidPos s) → Prop where
+  | last {i p j p' update} (step : Step nfa lb i p j p' update) : Path nfa lb i p j p' (List.ofOption update)
+  | more {i p j p' k p'' update updates} (step : Step nfa lb i p j p' update) (rest : Path nfa lb j p' k p'' updates) :
+    Path nfa lb i p k p'' (update ::ₒ updates)
 
 namespace Path
 
-variable {nfa nfa' : NFA} {lb lb' i it j it' k it'' updates updates₁ updates₂}
+variable {s : String} {nfa nfa' : NFA} {lb lb'} {p p' p'' : ValidPos s} {i j k updates updates₁ updates₂}
 
-theorem ge (path : nfa.Path lb i it j it' updates) : lb ≤ i := by
+theorem ge (path : nfa.Path lb i p j p' updates) : lb ≤ i := by
   cases path with
   | last step => exact step.ge
   | more step => exact step.ge
 
-theorem lt (path : nfa.Path lb i it j it' updates) : i < nfa.nodes.size := by
+theorem lt (path : nfa.Path lb i p j p' updates) : i < nfa.nodes.size := by
   cases path with
   | last step => exact step.lt
   | more step => exact step.lt
 
-theorem lt_right (wf : nfa.WellFormed) (path : nfa.Path lb i it j it' updates) : j < nfa.nodes.size := by
+theorem lt_right (wf : nfa.WellFormed) (path : nfa.Path lb i p j p' updates) : j < nfa.nodes.size := by
   induction path with
   | last step => exact step.lt_right wf
   | more _ _ ih => exact ih
 
-theorem toString (path : nfa.Path lb i it j it' updates) : it'.toString = it.toString := by
+theorem le (path : nfa.Path lb i p j p' updates) : p ≤ p' := by
   induction path with
-  | last step => exact step.toString_eq
-  | more step _ ih => exact step.toString_eq ▸ ih
-
-theorem le_pos (path : nfa.Path lb i it j it' updates) : it.pos ≤ it'.pos := by
-  induction path with
-  | last step => exact step.le_pos
-  | more step _ ih => exact Nat.le_trans step.le_pos ih
-
-theorem validL (path : nfa.Path lb i it j it' updates) : it.Valid := by
-  cases path with
-  | last step => exact step.validL
-  | more step => exact step.validL
-
-theorem validR (path : nfa.Path lb i it j it' updates) : it'.Valid := by
-  induction path with
-  | last step => exact step.validR
-  | more _ _ ih => exact ih
+  | last step => exact step.le
+  | more step _ ih => exact ValidPos.le_trans step.le ih
 
 /--
 A simpler casting procedure where the equality can be proven easily, e.g., when casting to a larger NFA.
 -/
 theorem cast (eq : ∀ i, lb ≤ i → (_ : i < nfa.nodes.size) → ∃ _ : i < nfa'.nodes.size, nfa[i] = nfa'[i])
-  (path : nfa.Path lb i it j it' updates) :
-  nfa'.Path lb i it j it' updates := by
+  (path : nfa.Path lb i p j p' updates) :
+  nfa'.Path lb i p j p' updates := by
   induction path with
   | last step =>
     have ⟨_, eq⟩ := eq _ step.ge step.lt
@@ -261,8 +176,8 @@ A casting procedure that transports a path from a larger NFA to a smaller NFA.
 -/
 theorem cast' (lt : i < nfa.nodes.size) (size_le : nfa.nodes.size ≤ nfa'.nodes.size) (wf : nfa.WellFormed)
   (eq : ∀ i, lb ≤ i → (lt : i < nfa.nodes.size) → nfa'[i]'(Nat.lt_of_lt_of_le lt size_le) = nfa[i])
-  (path : nfa'.Path lb i it j it' updates) :
-  nfa.Path lb i it j it' updates := by
+  (path : nfa'.Path lb i p j p' updates) :
+  nfa.Path lb i p j p' updates := by
   induction path with
   | last step => exact .last (step.cast (eq _ step.ge lt))
   | more step _ ih =>
@@ -270,22 +185,22 @@ theorem cast' (lt : i < nfa.nodes.size) (size_le : nfa.nodes.size ≤ nfa'.nodes
     have rest := ih (step.lt_right wf)
     exact .more step rest
 
-theorem liftBound (le : lb' ≤ lb) (path : nfa.Path lb i it j it' updates) :
-  nfa.Path lb' i it j it' updates := by
+theorem liftBound (le : lb' ≤ lb) (path : nfa.Path lb i p j p' updates) :
+  nfa.Path lb' i p j p' updates := by
   induction path with
   | last step => exact .last (step.liftBound le)
   | more step _ ih => exact .more (step.liftBound le) ih
 
 theorem liftBound' (ge : lb' ≤ i)
-  (inv : ∀ {i it j it' update}, lb' ≤ i → lb ≤ j → nfa.Step lb i it j it' update → lb' ≤ j)
-  (path : nfa.Path lb i it j it' updates) :
-  nfa.Path lb' i it j it' updates := by
+  (inv : ∀ {p p' : ValidPos s} {i j update}, lb' ≤ i → lb ≤ j → nfa.Step lb i p j p' update → lb' ≤ j)
+  (path : nfa.Path lb i p j p' updates) :
+  nfa.Path lb' i p j p' updates := by
   induction path with
   | last step => exact .last (step.liftBound' ge)
   | more step rest ih => exact .more (step.liftBound' ge) (ih (inv ge rest.ge step))
 
-theorem trans (path₁ : nfa.Path lb i it j it' updates₁) (path₂ : nfa.Path lb j it' k it'' updates₂) :
-  nfa.Path lb i it k it'' (updates₁ ++ updates₂) := by
+theorem trans (path₁ : nfa.Path lb i p j p' updates₁) (path₂ : nfa.Path lb j p' k p'' updates₂) :
+  nfa.Path lb i p k p'' (updates₁ ++ updates₂) := by
   induction path₁ with
   | last step =>
     simp
@@ -294,8 +209,8 @@ theorem trans (path₁ : nfa.Path lb i it j it' updates₁) (path₂ : nfa.Path 
     simp
     exact .more step (ih path₂)
 
-theorem compile_liftBound {e nfa} (eq : compile e = nfa) (path : nfa.Path 0 i it j it' updates) :
-  nfa.Path 1 i it j it' updates := by
+theorem compile_liftBound {e nfa} (eq : compile e = nfa) (path : nfa.Path 0 i p j p' updates) :
+  nfa.Path 1 i p j p' updates := by
   induction path with
   | last step => exact .last (step.compile_liftBound eq)
   | more step _ ih => exact .more (step.compile_liftBound eq) ih
@@ -303,7 +218,7 @@ theorem compile_liftBound {e nfa} (eq : compile e = nfa) (path : nfa.Path 0 i it
 /--
 If a property is closed under a single step, then it is closed under a path.
 -/
-theorem of_step_closure {lb} (motive : Nat → Iterator → Prop) (closure : ∀ i it j it' update, motive i it → nfa.Step lb i it j it' update → motive j it')
+theorem of_step_closure {lb} (motive : Nat → ValidPos s → Prop) (closure : ∀ i p j p' update, motive i p → nfa.Step lb i p j p' update → motive j p')
   {i it j it' update} (base : motive i it) (path : nfa.Path lb i it j it' update) :
   motive j it' := by
   induction path with
